Add fine-grained lock enforcement to semantics
Semantics enforces a StateR across yield points and a LockR at every
write, as well as corresponding StateI and LockI. The LockR/LockI are
intended solely for enforcing that every program respects locks for
every write, so that async reads can trust that the locking protocol is
followed.

To make writes (Assgn/Write) work with Commit, it is now required that
writes are _preceded_ by a Commit that respects the lock discipline
(that is, modifies the ghost copy when it is allowed to do so). All the
code has been updated to do so. Commit will eventually be renamed so
this pattern doesn't look odd.

Writeback has some issue with the intermediate Write not respecting the
cache LockI. This is due to the cache enforcing the fairly sophisticated
policy that the virtual disk reflect the disk + ghost cache, which is
probably not necessary. It should work out in this case regardless,
although might require an additional Commit.

src/ConcurrentCache.v
@@ -109,6 +109,8 @@ Definition lock_protects (lvar : var Scontents MutexOwner)
     tid <> owner_tid ->
     get v s' = get v s.
 
+Hint Unfold lock_protects : prog.
+
 Inductive lock_protocol (lvar : var Scontents MutexOwner) (tid : ID) :  S -> S -> Prop :=
 | NoChange : forall s s', get lvar s  = get lvar s' ->
                      lock_protocol lvar tid s s'
@@ -127,15 +129,18 @@ Hypothesis diskR_stutter : forall vd, diskR vd vd.
 
 Hint Resolve diskR_stutter.
 
-Definition cacheR tid : Relation S :=
+Definition cacheR (_:ID) : Relation S :=
   fun s s' =>
-    lock_protocol GCacheL tid s s' /\
-    lock_protects GCacheL GCache tid s s' /\
-    lock_protects GCacheL GDisk tid s s' /\
     let vd := virt_disk s in
     let vd' := virt_disk s' in
     (forall a v, vd a = Some v -> exists v', vd' a = Some v') /\
     diskR vd vd'.
+
+Definition lockR tid : Relation S :=
+  fun s s' =>
+    lock_protocol GCacheL tid s s' /\
+    lock_protects GCacheL GCache tid s s' /\
+    lock_protects GCacheL GDisk tid s s'.
 
 Inductive ghost_lock_invariant
           (lvar : var Mcontents Mutex)
@@ -148,7 +153,10 @@ Inductive ghost_lock_invariant
 
 Hint Constructors ghost_lock_invariant.
 
-Definition cacheI : Invariant Mcontents S :=
+Definition stateI : Invariant Mcontents S :=
+  fun m s d => True.
+
+Definition lockI : Invariant Mcontents S :=
   fun m s d =>
     let c := get Cache m in
     (d |= cache_pred c (virt_disk s))%judgement /\
@@ -156,13 +164,21 @@ Definition cacheI : Invariant Mcontents S :=
     (* mirror cache for sake of lock_protects *)
     get Cache m = get GCache s.
 
+Definition cacheI : Invariant Mcontents S :=
+  fun m s d =>
+    stateI m s d /\
+    lockI m s d.
+
 (* for now, we don't have any lemmas about the lock semantics so just operate
 on the definitions directly *)
 Hint Unfold lock_protects : prog.
-Hint Unfold cacheR cacheI : prog.
+Hint Unfold cacheR cacheI stateI lockI : prog.
 
 Ltac solve_get_set :=
   simpl_get_set;
+  try lazymatch goal with
+  | [ H: context[get _ (set _ _ _)] |- _ ] => progress (simpl_get_set in H)
+  end;
   try match goal with
       | [ |- _ =p=> _ ] => cancel
       | [ |- ?p _ ] => match type of p with
@@ -190,13 +206,13 @@ Ltac dispatch :=
       end.
 
 Definition cacheS : transitions Mcontents S :=
-  Build_transitions cacheR cacheI.
+  Build_transitions cacheR lockR stateI lockI.
 
 Hint Rewrite get_set.
 
 Ltac valid_match_opt :=
   match goal with
-  | [ |- valid _ _ _ _ (match ?discriminee with
+  | [ |- valid _ _ _ _ _ _ (match ?discriminee with
                        | _ => _
                        end) ] =>
     case_eq discriminee; intros;
@@ -224,19 +240,18 @@ Ltac inv_protocol :=
 
 Lemma cache_readonly' : forall tid s s',
     get GCacheL s = Owned tid ->
-    othersR cacheR tid s s' ->
+    othersR lockR tid s s' ->
     get GCache s' = get GCache s /\
     get GCacheL s' = Owned tid.
 Proof.
-  repeat (autounfold with prog).
-  unfold othersR.
+  unfold lockR, othersR.
   intros.
   deex; eauto; inv_protocol.
 Qed.
 
 Lemma cache_readonly : forall tid s s',
     get GCacheL s = Owned tid ->
-    star (othersR cacheR tid) s s' ->
+    star (othersR lockR tid) s s' ->
     get GCache s' = get GCache s /\
     get GCacheL s' = Owned tid.
 Proof.
@@ -247,19 +262,18 @@ Qed.
 
 Lemma virt_disk_readonly' : forall tid s s',
     get GCacheL s = Owned tid ->
-    othersR cacheR tid s s' ->
+    othersR lockR tid s s' ->
     get GDisk s' = get GDisk s /\
     get GCacheL s' = Owned tid.
 Proof.
-  repeat (autounfold with prog).
-  unfold othersR.
+  unfold lockR, othersR.
   intros.
   deex; eauto; inv_protocol.
 Qed.
 
 Lemma virt_disk_readonly : forall tid s s',
     get GCacheL s = Owned tid ->
-    star (othersR cacheR tid) s s' ->
+    star (othersR lockR tid) s s' ->
     get GDisk s' = get GDisk s /\
     get GCacheL s' = Owned tid.
 Proof.
@@ -403,9 +417,6 @@ Ltac cleanup :=
           || simpl_match);
   try congruence.
 
-Hint Extern 4 (get _ (set _ _ _) = _) => simpl_get_set : prog.
-Hint Extern 4 (_ = get _ (set _ _ _)) => simpl_get_set : prog.
-
 Ltac mem_contents_eq :=
   match goal with
   | [ H: get ?m ?var = _, H': get ?m ?var = _ |- _ ] =>
@@ -460,10 +471,19 @@ Ltac star_diskR := match goal with
                               cbn in H)
                    end.
 
+Check sectors_unchanged.
+
+Ltac sector_unchanged :=
+  match goal with
+  | [ H: forall a v, ?vd a = Some v -> (exists _, _), H': ?vd ?a = Some ?v |- _ ] =>
+    learn_fact (H a v H')
+  end.
+
 Ltac learn_invariants :=
   try cache_locked;
   try disk_locked;
   try sectors_unchanged;
+  try sector_unchanged; repeat deex;
   try star_diskR.
 
 (** These proofs are still very messy. There's a lot of low-level
@@ -961,6 +981,7 @@ Ltac simplify :=
   cleanup.
 
 Ltac finish :=
+  simpl_goal;
   solve_get_set;
   try solve [ pred_apply; cancel ];
   try cache_contents_eq;
@@ -1061,12 +1082,22 @@ Definition locked_disk_read {T} a rx : prog Mcontents S T :=
   match cache_get c a with
   | None => v <- Read a;
       let c' := cache_add c a v in
-      Assgn Cache c';;
-            Commit (set GCache c');;
+      Commit (set GCache c');;
+             Assgn Cache c';;
             rx v
   | Some (_, v) =>
     rx v
   end.
+
+Lemma ghost_lock_owned : forall lvar glvar m s tid,
+    ghost_lock_invariant lvar glvar m s ->
+    get glvar s = Owned tid ->
+    get lvar m = Locked.
+Proof.
+  inversion 1; congruence.
+Qed.
+
+Hint Resolve ghost_lock_owned.
 
 Theorem locked_disk_read_ok : forall a,
     cacheS TID: tid |-
@@ -1117,11 +1148,10 @@ Definition locked_async_disk_read {T} a rx : prog Mcontents S T :=
   c <- Get Cache;
   match cache_get c a with
   | None => v <- Read a;
-      Commit (set GCache c);;
              Yield;;
              let c' := cache_add c a v in
+             Commit (fun (s:S) => set GCache c' s);;
              Assgn Cache c';;
-                   Commit (fun (s:S) => set GCache c' s);;
                    rx v
   | Some (_, v) =>
     rx v
@@ -1160,8 +1190,24 @@ Proof.
   learn_some_addr.
   valid_match_opt; hoare pre simplify with (finish;
                                              try (replace_cache; vd_locked);
-                                             repeat unify_mem_contents;
                                              eauto).
+
+  eapply cache_pred_stable_add; eauto.
+  replace (get GDisk s1); eauto.
+  match goal with
+  | [ H: cache_pred ?c ?vd ?d |- cache_pred ?c' ?vd' ?d ] =>
+    replace c' with c by congruence;
+      replace vd' with vd by congruence;
+      eauto
+  end.
+  eapply cache_pred_stable_add; eauto.
+  replace (get GDisk s1); eauto.
+  match goal with
+  | [ H: cache_pred ?c ?vd ?d |- cache_pred ?c' ?vd' ?d ] =>
+    replace c' with c by congruence;
+      replace vd' with vd by congruence;
+      eauto
+  end.
 Qed.
 
 Hint Extern 4 {{locked_async_disk_read _; _}} => apply locked_async_disk_read_ok.
@@ -1169,9 +1215,9 @@ Hint Extern 4 {{locked_async_disk_read _; _}} => apply locked_async_disk_read_ok
 Definition disk_read {T} a rx : prog _ _ T :=
   AcquireLock CacheL (fun tid => set GCacheL (Owned tid));;
               v <- locked_async_disk_read a;
-  Assgn CacheL Open;;
-        Commit (set GCacheL NoOwner);;
-        rx v.
+  Commit (set GCacheL NoOwner);;
+         Assgn CacheL Open;;
+         rx v.
 
 Lemma cache_pred_same_sectors : forall c vd d,
     cache_pred c vd d ->
@@ -1221,7 +1267,7 @@ Theorem disk_read_ok : forall a,
 Proof.
   intros.
   step pre simplify with finish.
-  unfold cacheR; eauto.
+
   learn_some_addr.
   step pre (cbn; intuition; repeat deex;
             learn_invariants) with idtac.
@@ -1265,22 +1311,22 @@ Definition replace_latest vs v' :=
 Definition locked_disk_write {T} a v rx : prog Mcontents S T :=
   c <- Get Cache;
   let c' := cache_add_dirty c a v in
-  Assgn Cache c';;
-        Commit (set GCache c');;
-        Commit (fun (s:S) => let vd := get GDisk s in
-                           let rest := match (vd a) with
-                                       | Some (Valuset v0 rest) =>
-                                         match (cache_get c a) with
-                                         | Some (true, _) => rest
-                                         | Some (false, _) => v0 :: rest
-                                         | None => v0 :: rest
-                                         end
-                                       (* impossible *)
-                                       | None => nil
-                                       end in
-                           let vs' := Valuset v rest in
-                           set GDisk (upd vd a vs') s);;
-        rx tt.
+  Commit (set GCache c');;
+         Commit (fun (s:S) => let vd := get GDisk s in
+                            let rest := match (vd a) with
+                                        | Some (Valuset v0 rest) =>
+                                          match (cache_get c a) with
+                                          | Some (true, _) => rest
+                                          | Some (false, _) => v0 :: rest
+                                          | None => v0 :: rest
+                                          end
+                                        (* impossible *)
+                                        | None => nil
+                                        end in
+                            let vs' := Valuset v rest in
+                            set GDisk (upd vd a vs') s);;
+         Assgn Cache c';;
+         rx tt.
 
 Theorem locked_disk_write_ok : forall a v,
     cacheS TID: tid |-
@@ -1293,19 +1339,26 @@ Theorem locked_disk_write_ok : forall a v,
                             cacheI m' s' d' /\
                             get GCacheL s = Owned tid /\
                             exists rest', vd' |= F * a |-> (Valuset v rest') /\
-                            s0' = s0
+                                     s0' = s0
     }} locked_disk_write a v.
 Proof.
-  hoare pre (simplify; learn_some_addr) with finish.
-  case_cache_val;
-    cbn; try cache_vd_val; repeat deex; cleanup; eauto.
+  intros.
+  hoare pre (simplify; learn_some_addr) with
+    (finish;
+    try match goal with
+    | [ |- lock_protects _ _ _ _ _ ] =>
+      unfold lock_protects; intros; solve_get_set; try congruence
+    | [ |- cache_pred (cache_add_dirty _ _ _) (upd _ _ _) _ ] =>
+      case_cache_val;
+        cbn; try cache_vd_val; repeat deex;
+        cleanup; eauto
+    end).
 
   eapply pimpl_apply;
     [ | eapply ptsto_upd ];
     dispatch.
 Qed.
 
-(** Eviction, so far without writeback *)
 Definition evict {T} a rx : prog Mcontents S T :=
   c <- Get Cache;
   match cache_get c a with
@@ -1315,15 +1368,15 @@ Definition evict {T} a rx : prog Mcontents S T :=
          rx tt
        } else {
     let c' := cache_evict c a in
-    Assgn Cache c';;
-          Commit (set GCache c');;
+    Commit (set GCache c');;
+          Assgn Cache c';;
           rx tt
   }
 end.
 
 Ltac if_ok :=
   match goal with
-  | [ |- valid _ _ _ _ (If_ ?b _ _) ] =>
+  | [ |- valid _ _ _ _ _ _ (If_ ?b _ _) ] =>
     unfold If_; case_eq b; intros
   end.
 
@@ -1367,9 +1420,9 @@ Definition writeback {T} a rx : prog Mcontents S T :=
   | Some (true, v) =>
     Write a v;;
           let c' := cache_clean c a in
-          Assgn Cache c';;
-                Commit (set GCache c');;
-                rx tt
+          Commit (set GCache c');;
+                 Assgn Cache c';;
+                 rx tt
   | Some (false, _) => rx tt
   | None => rx tt
   end.
@@ -1492,7 +1545,7 @@ Theorem writeback_ok : forall a,
                      get GCacheL s = Owned tid /\
                      vd |= F * a |-> (Valuset v0 rest)
      | POST d' m' s0' s' _: let vd' := virt_disk s' in
-                            d' |= cache_pred (get Cache m') vd' /\
+                            cacheI m' s' d' /\
                             get GCacheL s = Owned tid /\
                             vd' = virt_disk s /\
                             s0' = s0
@@ -1509,12 +1562,17 @@ Proof.
   case_cache_val' (get Cache m) a;
     try cache_vd_val; repeat deex; cleanup.
 
-  all: valid_match_opt; hoare pre simplify with finish.
-  learn_some_addr.
+  all: valid_match_opt; hoare pre (simplify; learn_some_addr) with finish.
+  (* precondition of Write demands this; need to try proving it to see
+if it's true (otherwise, need to Commit a change to vd, Write, then
+Commit back to the original vd.) *)
+  admit.
+
   pred_apply; cancel.
   eapply pimpl_trans; [ | eapply cache_pred_clean' ]; eauto.
   cancel; eauto.
 
-  Grab Existential Variables.
-  all: auto.
-Qed.
+  pred_apply; cancel.
+  eapply pimpl_trans; [ | eapply cache_pred_clean' ]; eauto.
+  cancel; eauto.
+Admitted.
